theories/examples/latch/latch.c
@@ -1,0 +1,10 @@
+#include <stdbool.h>
+#include "latch.h"
+
+void latch_wait(struct latch* latch) {
+  while(atomic_load(&latch->released) == (_Bool)false) {}
+}
+
+void latch_release(struct latch* latch) {
+  atomic_store(&latch->released, true);
+}
