theories/examples/latch/latch_proof_latch_release.v
@@ -1,0 +1,26 @@
+From refinedc.typing Require Import typing.
+From refinedc.examples.latch Require Import latch_code.
+From refinedc.examples.latch Require Import latch_spec.
+From refinedc.examples.latch Require Import latch_def.
+Set Default Proof Using "Type".
+
+(* Generated from [theories/examples/latch/latch.c]. *)
+Section proof_latch_release.
+  Context `{!typeG Σ} `{!globalG Σ}.
+
+  (* Typing proof for [latch_release]. *)
+  Lemma type_latch_release :
+    ⊢ typed_function impl_latch_release type_of_latch_release.
+  Proof.
+    start_function "latch_release" ([[p beta] P]) => arg_latch.
+    split_blocks ((
+      ∅
+    )%I : gmap block_id (iProp Σ)) ((
+      ∅
+    )%I : gmap block_id (iProp Σ)).
+    - repeat liRStep; liShow.
+      all: print_typesystem_goal "latch_release" "#0".
+    Unshelve. all: prepare_sideconditions; normalize_and_simpl_goal; try solve_goal.
+    all: print_sidecondition_goal "latch_release".
+  Qed.
+End proof_latch_release.
